Improve Kappa notation and add equivalences (#93)

cava/cava/Cava/Arrow/Arrow.v
@@ -1,11 +1,17 @@
 From Coq Require Import Bool.Bvector.
 From Coq Require Import Bool.Bool.
+From Coq Require Import Setoid.
+From Coq Require Import Classes.Morphisms.
 
 From Cava Require Import Netlist.
 
-Reserved Infix "~>" (at level 90, right associativity).
+Reserved Infix "~>" (at level 90, no associativity).
+Reserved Infix "~[ C ]~>" (at level 90, no associativity).
+Reserved Infix ">>>" (at level 53, right associativity).
+Reserved Infix "=M=" (at level 54, no associativity).
+Reserved Infix "~O~" (at level 54, no associativity).
+
 Reserved Infix "**" (at level 30, right associativity).
-Reserved Infix ">>>" (at level 90, right associativity).
 
 (* more flexible than a haskell style category,
   which has morphisms between objects of type Hask.
@@ -21,21 +27,52 @@ Class Category := {
 
   compose {x y z} (f: y ~> z) (g : x ~> y) : x ~> z
     where "g >>> f" := (compose f g);
+
+  (* Setoid equivalence *)
+
+  morphism_equivalence: forall x y (f g: x ~> y), Prop
+    where "f =M= g" := (morphism_equivalence _ _ f g);
+  morphism_setoid_equivalence : forall x y , Equivalence (morphism_equivalence x y);
+  compose_respects_equivalence : forall x y z , Proper (morphism_equivalence y z ==> morphism_equivalence x y ==> morphism_equivalence x z) compose;
+
+  (* Laws, used in rewriting *)
+
+  id_left {x y} (f: x ~> y) : (id >>> f) =M= f;
+  id_right {x y} (f: x ~> y) : (f >>> id) =M= f;
+
+  associativity {x y z w} {f: x~>y} {g: y~>z} {h: z~>w} : (f >>> g) >>> h =M= f >>> (g >>> h);
 }.
 
 Declare Scope category_scope.
 Bind Scope category_scope with Category.
 Delimit Scope category_scope with category.
 
-Notation "x ~> y" := (morphism x y)
-  (at level 90, right associativity) : category_scope.
-Notation "x ~[ C ]~> y" := (@morphism C x y)
-  (at level 90) : category_scope.
-Notation "g >>> f" := (compose f g)
-  (at level 90, right associativity) : category_scope.
+Notation "x ~> y" := (morphism x y) : category_scope.
+Notation "x ~[ C ]~> y" := (@morphism C x y) (at level 90): category_scope.
+Notation "g >>> f" := (compose f g) : category_scope.
+Notation "f =M= g" := (morphism_equivalence _ _ f g) : category_scope.
+(* Notation "x ~O~ y" := (object_equivalence x y) : category_scope. *)
 
 Open Scope category_scope.
-Print Category.
+
+Add Parametric Relation (C: Category) (x y: object): (morphism x y) (morphism_equivalence x y)
+  reflexivity proved by  (@Equivalence_Reflexive  _ _ (morphism_setoid_equivalence x y))
+  symmetry proved by     (@Equivalence_Symmetric  _ _ (morphism_setoid_equivalence x y))
+  transitivity proved by (@Equivalence_Transitive _ _ (morphism_setoid_equivalence x y))
+  as parametric_relation_eqv.
+
+Hint Extern 1 => apply compose_respects_equivalence: core.
+Hint Extern 1 => apply id_left: core.
+Hint Extern 1 => apply id_right: core.
+
+Add Parametric Morphism (C: Category) (x y z: object) : (@compose C x y z)
+  with signature (morphism_equivalence _ _ ==> morphism_equivalence _ _ ==> morphism_equivalence _ _) 
+  as parametric_morphism_comp.
+Proof. auto. Defined.
+
+(* This is the same as passing a pair type to 'sig', but is more convinent to use. *)
+Inductive sig_pair (A B:Type) (P:A -> B -> Prop) : Type :=
+  exist_pair : forall (x:A) (y:B), P x y -> sig_pair A B P.
 
 (* adam megacz style arrow;
   There is no method to provide lifting a Coq function in general,
@@ -51,7 +88,9 @@ Class Arrow := {
   drop {x} : x ~> unit;
   swap {x y} : x**y ~> y**x;
 
-  fork {x y z} (f : x ~> y) (g : x ~> z) : x ~> y ** z;
+  first {x y z} (f : x ~> y) : x ** z ~> y ** z;
+  second {x y z} (f : x ~> y) : z ** x ~> z ** y;
+
   exl  {x y} : x ** y ~> x;
   exr  {x y} : x ** y ~> y;
 
@@ -59,7 +98,29 @@ Class Arrow := {
   uncancelr {x} : x ~> x**unit;
   assoc {x y z} : ((x**y)**z) ~> (x**(y**z));
   unassoc {x y z} : (x**(y**z)) ~> ((x**y)**z);
+
+  (* laws, currently somewhat ad-hoc*)
+
+  obj_equiv x y := 
+    (sig_pair (x~>y) (y~>x) (fun f g => 
+    f >>> g =M= id /\
+    g >>> f =M= id
+    ));
+
+  exl_unit_uncancelr x : @exl x unit >>> uncancelr =M= id;
+  exr_unit_uncancell x : @exr unit x >>> uncancell =M= id;
+  uncancelr_exl x : uncancelr >>> @exl x unit =M= id;
+  uncancell_exr x : uncancell >>> @exr unit x =M= id;
+
+  drop_annhilates : forall x y (f: x~>y), f >>> drop =M= drop;
+  exl_unit_is_drop : forall x, @exl unit x =M= drop;
+  exr_unit_is_drop : forall x, @exr x unit =M= drop;
+
+  exl_unit x : obj_equiv (x**unit) x;
+  prefix_equiv x y : obj_equiv x y -> forall a, obj_equiv (a**x) (a**y);
 }.
+
+Coercion cat: Arrow >-> Category.
 
 Declare Scope arrow_scope.
 Bind Scope arrow_scope with Arrow.
@@ -70,11 +131,23 @@ Notation "x ** y" := (product x y)
 
 Open Scope arrow_scope.
 
-Definition first {_: Arrow} {x y z} (f : x ~> y) : x ** z ~> y ** z :=
-  fork (exl >>> f) exr.
+Definition apply_object_equivalence_left: forall (arr:Arrow) x y (H: obj_equiv x y), x~>y.
+Proof.
+  intros.
+  inversion H.
+  exact x0.
+Defined.
 
-Definition second {_: Arrow} {x y z} (f : x ~> y) : z ** x ~> z ** y :=
-  fork exl (exr >>> f).
+Definition apply_object_equivalence_right: forall (arr:Arrow) x y (H: obj_equiv x y), y~>x.
+Proof.
+  intros.
+  inversion H.
+  exact y0.
+Defined.
+
+Ltac resolve_object_equivalence :=
+  try repeat refine (prefix_equiv _ _ _ _);
+  exact (exl_unit _).
 
 (* Loop as a different type class to allow implementating a subset of features *)
 Class ArrowLoop (A: Arrow) := {
@@ -82,11 +155,9 @@ Class ArrowLoop (A: Arrow) := {
   loopl {x y z} : (z**x ~> z**y) -> (x ~> y);
 }.
 
-Print Arrow.
-
 (* Cava *)
 Class Cava  := {
-  cava_arr :> Arrow;
+  cava_arrow :> Arrow;
 
   bit : object;
   bitvec : nat -> object;
@@ -109,6 +180,8 @@ Class Cava  := {
   unsigned_add a b s: bitvec a ** bitvec b ~> bitvec s;
 }.
 
+Coercion cava_arrow: Cava >-> Arrow.
+
 Definition cava_cat (_: Cava): Category := _.
 Definition cava_obj (cava: Cava): Type := @object (@cava_cat cava).
 
@@ -120,5 +193,7 @@ Class CavaDelay := {
   delay_cava :> Cava;
   delay_gate {x} : x ~> x;
 }.
+
+Coercion delay_cava: CavaDelay >-> Cava.
 
 Definition cava_delay_arr (_: CavaDelay): Arrow := _.
