cava/cava/Cava/Arrow/Syntax.v
@@ -1,44 +1,143 @@
 Require Export Cava.Arrow.Syntax.Kappa.
 Require Export Cava.Arrow.Syntax.Desugared.
 Require Export Cava.Arrow.Syntax.CC.
+Require Export Cava.Arrow.Instances.Combinational.
 
 Require Import Cava.Arrow.Arrow.
 Require Import Cava.BitArithmetic.
 
+Require Import Arith Eqdep List Lia.
+
 (* Notations *)
 
-Declare Scope source_scope.
+Require Import List Lia.
+Import ListNotations.
+
+Declare Scope expression_scope.
 Declare Custom Entry expr.
-Delimit Scope source_scope with source.
+Delimit Scope expression_scope with source.
 
 Notation "<[ e ]>" := (
-  Desugar _ (fun var => e)
-  ) (at level 1, e custom expr at level 1): source_scope.
-Notation "\ x => e" := (Abs (fun x => e)) (in custom expr at level 1, x constr at level 4, e custom expr at level 4): source_scope.
+  Desugar _ (fun var => 
+    e%source 
+  )
+  ) (at level 1, e custom expr at level 1).
 
-(* TODO: is this bugged?
-Notation "\ x .. y => e" :=
-  (Abs (fun x =>  ..
-  (Abs (fun y => e)) ..
-  ))
-  (in custom pat at level 1, x constr at level 4, e custom expr at level 4): source_scope. *)
+Notation "\ x .. y => e" := (Abs (fun x => .. (Abs (fun y => e)) ..))
+  (in custom expr at level 200, x binder, right associativity,
+   format "'[' \  '/  ' x  ..  y =>  '/  ' e ']'")
+                                  : expression_scope.
 
-Notation "x y" := (App x y) (in custom expr at level 3, left associativity).
-Notation "~~( x )" := (Arr x) (in custom expr, x constr).
-Notation "~!( x )" := (Arr (Closure_conversion x)) (in custom expr, x constr).
+Notation "x y" := (App x y) (in custom expr at level 3, left associativity) : expression_scope.
+Notation "~~( x )" := (Arr x) (in custom expr, x constr) : expression_scope.
+Notation "! x" := (Iso (Arr x) (ltac:( resolve_object_equivalence ))
+  ) (in custom expr at level 2, x global) : expression_scope.
+Notation "~!( x )" := (Arr (Closure_conversion x)) (in custom expr, x constr) : expression_scope.
 (* alternatively *)
 (* Notation "~!( x )" := (kappa_reinject _ (x _)) (in custom expr, x constr). *)
 
-Notation "'let' x = e1 'in' e2" := (Let e1 (fun x => e2)) (in custom expr at level 1, x constr at level 4, e2 at level 5, e1 at level 1).
-Notation "x" := (Var x) (in custom expr, x ident).
-Notation "( x )" := x (in custom expr, x at level 4).
+Notation "'let' x = e1 'in' e2" := (Let e1 (fun x => e2)) (in custom expr at level 1, x constr at level 4, e2 at level 5, e1 at level 1) : expression_scope.
+Notation "x" := (Var x) (in custom expr, x ident) : expression_scope.
+Notation "( x )" := x (in custom expr, x at level 4) : expression_scope.
 
-Notation "'fst' e" := (Compose (Arr exl) e) (in custom expr at level 4, e custom expr at level 4).
-Notation "'snd' e" := (Compose (Arr exr) e) (in custom expr at level 4, e custom expr at level 4). 
+Notation "( x , y )" := (
+    Com (Arr (unassoc >>> exl)) (App (App (Arr id) x) y) 
+    )
+   (in custom expr, x at level 4, y at level 4) : expression_scope.
 
-Notation "# x" := (Arr (constant x)) (in custom expr at level 2, x constr at level 4).
-Notation "#v x" := (Arr (constant_vec _ (nat_to_bitvec_sized _ x))) (in custom expr at level 2, x constr at level 4).
+Notation "'fst'' e" := (Com (Arr exl) e) (in custom expr at level 4, e custom expr at level 4) : expression_scope.
+Notation "'snd'' e" := (Com (Arr exr) e) (in custom expr at level 4, e custom expr at level 4) : expression_scope.
+
+Notation "# x" := (Arr (constant x)) (in custom expr at level 2, x constr at level 4) : expression_scope.
+Notation "#v x" := (Arr (constant_vec _ (nat_to_bitvec_sized _ x))) (in custom expr at level 2, x constr at level 4) : expression_scope.
 
 (* test notation *)
 
-Open Scope source_scope.
+Local Open Scope expression_scope.
+
+(* 1. simple constant *)
+Definition ex1_notation {cava: Cava}: Kappa (bit**unit) bit := <[ \ x => #true ]> .
+
+(* 2. branching on Coq value *)
+Definition ex2_notation {cava: Cava} (n:nat) : Kappa (bit**unit) bit :=
+match n with
+| O => <[ \ x => #true ]>
+| S n => <[ \ x => !xor_gate x x ]> 
+end.
+
+(* 3. adder tree *)
+Fixpoint make_obj `{Arrow} o (n:nat) :=
+match n with
+| O => o
+| S n => make_obj o n ** make_obj o n
+end.
+
+Fixpoint tree `{Cava} (A: object)
+  (n: nat)
+  (f: A**A ~> A)
+  {struct n}
+  : Kappa (make_obj A n ** unit) A :=
+match n with
+| O => <[ \x => x ]>
+| S n' => <[\x =>
+            let a = ~!(tree A n' f) (fst' x) in
+            let b = ~!(tree A n' f) (snd' x) in
+
+            !f a b
+            ]>
+end.
+
+Definition xilinxFullAdder `{Cava}
+  : Kappa (bit ** (bit ** bit) ** unit) (bit**bit) :=
+  <[ \ cin ab =>
+     let a = fst' ab in
+     let b = snd' ab in
+     let part_sum = !xor_gate a b in
+     let sum      = !xorcy part_sum cin in
+     let cout     = !muxcy part_sum cin a in
+     (sum, cout)
+  ]>.
+
+Definition xilinxFullAdder' := @Closure_conversion Combinational _ _ xilinxFullAdder .
+Definition xilinxFullAdder'' : bool := fst ((@Closure_conversion Combinational _ _ xilinxFullAdder) (true, ((true,true), tt))).
+
+Definition adder_tree `{Cava}
+  (bitsize: nat)
+  (n: nat)
+  : Kappa (make_obj (bitvec bitsize) n ** unit) (bitvec bitsize) :=
+  tree (bitvec bitsize) n (unsigned_add _ _ _).
+
+Notation "v : 'u' sz" := (constant_vec sz (nat_to_bitvec_sized sz v))
+  (only printing, at level 99, format "'[ ' v : 'u' sz ']'").
+
+Ltac unfold_notation :=
+  (unfold Desugar;
+  unfold desugar;
+  unfold Closure_conversion;
+  unfold closure_conversion
+  ).
+
+Lemma kappa_arrow_lemma_example:
+  forall (Cava: Cava),
+  Closure_conversion ex1_notation = (uncancelr >>> first swap >>> assoc >>> exl >>> constant true).
+Proof.
+  intros.
+  auto.
+Qed.
+
+Lemma kappa_arrow_lemma_example2:
+  forall (Cava: Cava),
+  Closure_conversion ex1_notation =M= (drop >>> constant true).
+Proof.
+  intros.
+  unfold_notation.
+  simpl.
+  setoid_rewrite exl_unit_is_drop.
+  setoid_rewrite <- associativity at 3.
+  setoid_rewrite drop_annhilates.
+  setoid_rewrite <- associativity at 2.
+  setoid_rewrite drop_annhilates.
+  setoid_rewrite <- associativity at 1.
+  setoid_rewrite drop_annhilates.
+  reflexivity.
+Qed.
