cava/cava/Cava/Arrow.v
@@ -1,6 +1,6 @@
 Require Export Cava.Arrow.Arrow.
-Require Export Cava.Arrow.Instances.Coq.
+Require Export Cava.Arrow.Instances.Combinational.
 Require Export Cava.Arrow.Instances.Netlist.
-Require Export Cava.Arrow.Instances.Stream.
+(* Require Export Cava.Arrow.Instances.Stream. *)
 
 Require Export Cava.Arrow.Syntax.
