cava/cava/Cava/Arrow/Instances/Combinational.v
@@ -1,0 +1,143 @@
+From Coq Require Import Bool.Bool.
+From Coq Require Import Bool.Bvector.
+
+Require Import Cava.BitArithmetic.
+Require Import Cava.Arrow.Arrow.
+
+From Coq Require Import Setoid.
+From Coq Require Import Classes.Morphisms.
+
+Require Import FunctionalExtensionality.
+
+(******************************************************************************)
+(* Evaluation as function evaluation, no delay elements or loops              *)
+(******************************************************************************)
+
+
+Section CoqEval.
+  #[refine] Instance CoqCat : Category := {
+    object := Type;
+    morphism X Y := X -> Y;
+    compose _ _ _ f g x := f (g x);
+    id X x := x;
+
+    morphism_equivalence x y f g := f = g;
+  }.
+  Proof.
+    intros.
+    unfold Proper. 
+    refine (fun f => _). intros.
+    refine (fun g => _). intros.
+    rewrite H.
+    rewrite H0.
+    auto.
+
+    auto.
+    auto.
+
+    auto.
+  Defined.
+
+  Ltac simple_destruct :=
+  match goal with
+  | [H: ?X * ?Y |- _] => destruct H
+  | [H: Datatypes.unit |- _] => destruct H
+  end.
+  Ltac simple_solve :=
+    intros; simpl; extensionality z; repeat simple_destruct; auto.
+
+  #[refine] Instance CoqArr : Arrow := {
+    cat := CoqCat;
+    unit := Datatypes.unit : Type ;
+    product := prod;
+
+    first _ _ _ f '(x, y) := (f x, y);
+    second _ _ _ f '(x, y) := (x, f y);
+    exl X Y := fst;
+    exr X Y := snd;
+
+    drop _ x := tt;
+    copy _ x := pair x x;
+
+    swap _ _ x := (snd x, fst x);
+
+    uncancell _ x := (tt, x);
+    uncancelr _ x := (x, tt);
+
+    assoc _ _ _ '((x,y),z) := (x,(y,z));
+    unassoc _ _ _ '(x,(y,z)) := ((x,y),z);
+  }.
+  Proof.
+    simple_solve.
+    simple_solve.
+    simple_solve.
+    simple_solve.
+    simple_solve.
+    simple_solve.
+    simple_solve.
+
+    intros.
+    refine (exist_pair (prod x Datatypes.unit~>x) (x~> prod x Datatypes.unit) _ fst (fun x => pair x tt)  _).
+    simpl.
+    split.
+    simple_solve.
+    auto.
+
+    intros.
+    inversion X.
+    inversion H.
+    inversion H0.
+    inversion H1.
+    refine (exist_pair (prod a x ~> prod a y) (prod a y ~> prod a x) _
+      (fun '(a,b) => (a, x0 b))
+      (fun '(a,b) => (a, y0 b))
+      _).
+    
+    simpl.
+    split.
+
+    - extensionality z.
+      destruct z.
+      f_equal.
+      apply (f_equal (fun f => f x1)) in H3.
+      auto.
+
+    - extensionality z.
+      destruct z.
+      f_equal.
+      apply (f_equal (fun f => f y1)) in H4.
+      auto.
+  Defined.
+
+  Instance Combinational : Cava := {
+    bit := bool;
+    bitvec n := Bvector n;
+
+    constant b _ := b;
+    constant_vec n v _ := v;
+
+    not_gate b := negb b;
+    and_gate '(x,y) := andb x y;
+    nand_gate '(x,y) := negb (andb x y);
+    or_gate '(x,y) := orb x y;
+    nor_gate '(x,y) := negb (orb x y);
+    xor_gate '(x,y) := xorb x y;
+    xnor_gate '(x,y) := negb (xorb x y);
+    buf_gate x := x;
+
+    xorcy '(x,y) := xorb x y;
+    muxcy '(i,(t,e)) := if i then t else e;
+
+    unsigned_add m n s '(av, bv) :=
+      let a := bitvec_to_nat av in
+      let b := bitvec_to_nat bv in
+      let c := a + b in
+      nat_to_bitvec_sized s c;
+  }.
+
+  Example not_true: not_gate true = false.
+  Proof. reflexivity. Qed.
+  Example not_false: not_gate false = true.
+  Proof. reflexivity. Qed.
+
+End CoqEval.
