cava/cava/Cava/Arrow/Syntax/Kappa.v
@@ -1,4 +1,10 @@
+Require Import List Lia.
+
+Import ListNotations.
+
 Require Import Cava.Arrow.Arrow.
+
+Reserved Infix "<-->" (at level 90, no associativity).
 
 Section WithArrow.
   Variable arr: Arrow.
@@ -7,56 +13,27 @@ Section WithArrow.
     Variable var: object -> object -> Type.
 
     Inductive kappa_sugared : object -> object -> Type :=
-    | Var : forall x y,     var x y -> kappa_sugared x y
-    | Abs : forall x y z,   (var unit x -> kappa_sugared y z) -> kappa_sugared (x**y) z
-    | App : forall x y z,   kappa_sugared (x**y) z -> kappa_sugared unit x -> kappa_sugared y z
-    | Compose : forall x y z, kappa_sugared y z -> kappa_sugared x y -> kappa_sugared x z
-    | Arr : forall x y,     morphism x y -> kappa_sugared x y
-    | Let : forall x y z,   kappa_sugared unit x -> (var unit x -> kappa_sugared y z) -> kappa_sugared y z .
+    | Var: forall x y,    var x y -> kappa_sugared x y
+    | Abs: forall x y z,  (var unit x -> kappa_sugared y z) -> kappa_sugared (x**y) z
+    | App: forall x y z,  kappa_sugared (x**y) z -> kappa_sugared unit x -> kappa_sugared y z
+    | Com: forall x y z,  kappa_sugared y z -> kappa_sugared x y -> kappa_sugared x z
+    | Arr: forall x y,    morphism x y -> kappa_sugared x y
+    | Let: forall x y z,  kappa_sugared unit x -> (var unit x -> kappa_sugared y z) -> kappa_sugared y z 
+    | Iso: forall x y z,  kappa_sugared y z -> obj_equiv x y -> kappa_sugared x z
+    .
   End Vars.
 
   Definition Kappa_sugared i o := forall var, @kappa_sugared var i o.
-
-  (* TODO: enable transforms? *)
-  (* Reserved Infix "<-->" (at level 90, no associativity). *)
-  (* Reserved Infix "≅" (at level 90, no associativity). *)
-  (* Reserved Infix "--->" (at level 90, no associativity). *)
-  (* (1* Non-destructive transform / isomorphism *1) *)
-  (* Inductive iso : object -> object -> Type := *)
-  (* | IId:          forall x,     x <--> x *)
-  (* | ICancelL:     forall x,     (unit ** x) <--> x *)
-  (* | ICancelR:     forall x,     (x ** unit) <--> x *)
-  (* | IUncancelL:   forall x,     x <--> (unit ** x) *)
-  (* | IUncancelR:   forall x,     x <--> (x ** unit) *)
-
-  (* | IAssociate:   forall x y z, ((x ** y) ** z) <--> (x ** (y ** z)) *)
-  (* | IUnassociate: forall x y z, (x ** (y ** z)) <--> ((x ** y) ** z) *)
-  (* where "x <--> y" := (iso x y). *)
-
-  (* Inductive iso_closure: object -> object -> Type := *)
-  (* | IIso:     forall x y,     x <--> y -> x ≅ y *)
-  (* | ICompose: forall x y z,   x <--> y -> y <--> z -> x ≅ z *)
-  (* (1* | IProduct: forall x y z w, x <--> y -> z <--> w -> x**z ≅ y**w *1) *)
-  (* where "x ≅ y" := (iso_closure x y). *)
-
-  (* (1* Destructive object re-arrangement rules *1) *)
-  (* Inductive arrange : object -> object -> Type := *)
-  (* | ALeft:    forall x z,   (z ** x) ---> x *)
-  (* | ARight:   forall x z,   (x ** z) ---> x *)
-  (* | AWeak:    forall x,     x ---> unit *)
-
-  (* | AIso:     forall x y,   x <--> y -> x ---> y *)
-  (* | ACompose: forall x y z, x ---> y -> y ---> z -> x ---> z *)
-  (* where "x ---> y" := (arrange x y). *)
 
 End WithArrow.
 
 Arguments Var [arr var x y].
 Arguments Abs [arr var x y z].
 Arguments App [arr var x y z].
-Arguments Compose [arr var x y z].
+Arguments Com [arr var x y z].
 Arguments Arr [arr var x y].
 Arguments Let [arr var x y z].
+Arguments Iso [arr var x y z].
 
 Arguments kappa_sugared [arr].
 Arguments Kappa_sugared [arr].
