cava/cava/Cava/Extraction.v
@@ -34,12 +34,14 @@ Recursive Extraction Library Combinators.
 
 Require Import Cava.Arrow.Arrow.
 Require Import Cava.Arrow.Syntax.
-Require Import Cava.Arrow.Instances.Coq.
+Require Import Cava.Arrow.Syntax.Desugared.
+Require Import Cava.Arrow.Syntax.CC.
+Require Import Cava.Arrow.Instances.Combinational.
 Require Import Cava.Arrow.Instances.Netlist.
 Recursive Extraction Library Arrow.
 Recursive Extraction Library Syntax.
 
-Recursive Extraction Library Coq.
+Recursive Extraction Library Combinational.
 Recursive Extraction Library Netlist.
 Recursive Extraction Library UnsignedAdders.
 Recursive Extraction Library XilinxAdder.
